LwRust/Paper.lean
@@ -1,6 +1,7 @@
+import LwRust.Paper.BorrowChecker
+import LwRust.Paper.Runtime
 import LwRust.Paper.InductiveSemantics
 import LwRust.Paper.StoreTyping
 import LwRust.Paper.Progress
 import LwRust.Paper.Preservation
-import LwRust.Paper.Adequacy
 import LwRust.Paper.Soundness
